pair

src/pca.lean
@@ -1,6 +1,5 @@
 import data.option.basic
 import tactic
---import data.real.basic
 
 universe variable u
 
@@ -12,6 +11,8 @@ infixl ` ⬝ ` := partial_magma.mul
 infix ` ↓= `:50 := λ x y, x = some y
 prefix `↓`:80 := some
 
+abbreviation defined  : option α →  bool := option.is_some
+
 def partial_magma.mmul [partial_magma α] : option α → option α → option α
 | ↓x ↓y := x ⬝ y
 | none _ := none
@@ -21,10 +22,10 @@ instance pm_mul [c : partial_magma α] : has_mul (option α) := {mul := @partial
 /- Partial Combinatory Algebra -/
 class pca (α : Type u) extends partial_magma α :=
 (k : α)
-(ktot : ∀ x, option.is_some (k ⬝ x))
+(ktot : ∀ x, defined (k ⬝ x))
 (k_constant : ∀ x y : α, k ⬝ x * y = x)
 (s : α)
-(stot : ∀ x y : α, option.is_some (s ⬝ x * y))
+(stot : ∀ x y : α, defined (s ⬝ x * y))
 (s_substitution : ∀ x y z : α, s ⬝ x * y * z = (x ⬝ z) * (y ⬝ z))
 
 def pca.equiv [partial_magma α] (a b : option α) : Prop := ∀ x : α, a * ↓x = b * ↓x
@@ -37,45 +38,28 @@ def subst [pca α] (x y : α) := option.get (stot x y)
 notation `𝐤` := const
 notation `𝐬` := subst
 
-lemma k_constant_ [c : pca α] : ∀ x y : α, k ⬝ x * ↓y = ↓x := c.k_constant
-lemma s_substitution_ [c : pca α] : ∀ x y z : α, s ⬝ x * ↓y * ↓z = (x ⬝ z) * (y ⬝ z) := c.s_substitution
-lemma s_substitution_0 [c : pca α] : ∀ x y z : α, ↓s * ↓x * ↓y * ↓z = (x ⬝ z) * (y ⬝ z) := c.s_substitution
-lemma k_compute [pca α] (x : α) : k ⬝ x = ↓(𝐤 x) := by { unfold const, simp }
-lemma s_compute [pca α] (x y : α) : s ⬝ x * ↓y = ↓(𝐬 x y) := by { unfold subst, simp, refl }
+@[simp] lemma k_simp [pca α] (a : α) : ↓k * ↓a = ↓(𝐤 a) := by { unfold const, simp, refl }
+@[simp] lemma s_simp [pca α] (a b : α) : ↓s * ↓a * ↓b = ↓(𝐬 a b) := by { unfold subst, simp, refl }
 
-
-lemma constant_simp [pca α] (a b : α) : 𝐤 a ⬝ b ↓= a :=
+@[simp]
+lemma k_simp0 [pca α] (a b : α) : ↓(𝐤 a) * ↓b = ↓a :=
 begin
-  have e : (k ⬝ a : option α) = ↓(𝐤 a), { unfold const, simp },
   calc
-    𝐤 a ⬝ b = k ⬝ a * ↓b : by { rw e, refl }
-    ...     = ↓a           : k_constant _ _
+    ↓(𝐤 a) * ↓b = ↓k * ↓a * ↓b : by { simp, }
+    ...           = ↓a             : k_constant _ _
 end
 
-lemma substitution_simp [pca α] (a b c : α) : 𝐬 a b ⬝ c = a ⬝ c * b ⬝ c :=
+@[simp] 
+lemma s_simp0 [pca α] (a b c : α) : ↓(𝐬 a b) * ↓c = (↓a * ↓c) * (↓b * ↓c) :=
 begin
-  have e : (s ⬝ a * ↓b : option α) = ↓(𝐬 a b), { unfold subst, simp, refl },
   calc
-    𝐬 a b ⬝ c = s ⬝ a * ↓b * ↓c : by { rw e, refl }
-    ...       = a ⬝ c * b ⬝ c           : s_substitution _ _ _
+    ↓(𝐬 a b) * ↓c = ↓s * ↓a * ↓b * ↓c : by { simp, }
+    ...             = a ⬝ c * b ⬝ c           : s_substitution _ _ _
 end
 
 def i [pca α] : α := 𝐬 k k
 
-lemma i_ident [pca α] (x : α) : i ⬝ x ↓= x :=
-begin
-  calc
-    i ⬝ x = (𝐬 k k) ⬝ x       : by { unfold i, }
-    ...   = k ⬝ x * k ⬝ x     : by { simp only [substitution_simp], }
-    ...   = k ⬝ x * (↓(𝐤 x)) : by { unfold const, simp, }
-    ...   = ↓x               : by { simp only [k_constant_], }
-end
-
-@[simp] lemma k_compute0 [pca α] (a : α) : ↓k * ↓a = ↓(𝐤 a) := k_compute a
-@[simp] lemma s_compute0 [pca α] (a b : α) : ↓s * ↓a * ↓b = ↓(𝐬 a b) := s_compute a b
-@[simp] lemma k_simp [pca α] (a b : α) : ↓(𝐤 a) * ↓b = ↓a := constant_simp a b
-@[simp] lemma s_simp [pca α] (a b c : α) : ↓(𝐬 a b) * ↓c = (↓a * ↓c) * (↓b * ↓c) := substitution_simp a b c
-@[simp] lemma i_simp [pca α ] (a : α) : ↓i * ↓a = ↓a := i_ident a
+@[simp] lemma i_ident [pca α] (a : α) : ↓i * ↓a = ↓a := by { unfold i, simp, }
 
 inductive lambda (α : Type u) [pca α]
 | var : ℕ → lambda
@@ -91,12 +75,12 @@ def lam [pca α] (n : ℕ) :lambda α → lambda α
 | (l * k) := (com s) * (lam l) * (lam k)
 notation `Λ`x`,` := lam x 
 
-def code [pca α] : lambda α → option α
+def expr [pca α] : lambda α → option α
 | (var x) := ↓k
 | (com c) := ↓c
-| (l * k) := (code l) * (code k)
+| (l * k) := (expr l) * (expr k)
 
-lemma lambda_defined [c : pca α] : ∀ (n : ℕ) (e : lambda α), option.is_some (code (Λ n, e) : option α)
+lemma lambda_defined [c : pca α] : ∀ (n : ℕ) (e : lambda α), defined (expr (Λ n, e) : option α)
 | n (var e) := begin
     cases (eq.decidable n e),
     { have he : (Λ n, (var e) : @lambda _ c) = com k * var e, { simp [lam], intros, contradiction },
@@ -108,23 +92,25 @@ lemma lambda_defined [c : pca α] : ∀ (n : ℕ) (e : lambda α), option.is_som
   end
 | n (com c) := ktot c
 | n (l * m) := begin
-    simp [lam, code], 
+    simp [lam, expr], 
     let a := option.get (lambda_defined n l),
     let b := option.get (lambda_defined n m),
-    have ha : code (Λ n, l) = ↓a, { simp },
-    have hb : code (Λ n, m) = ↓b, { simp },
+    have ha : expr (Λ n, l) = ↓a, { simp },
+    have hb : expr (Λ n, m) = ↓b, { simp },
     rw [ha, hb],
     exact stot a b
   end
 
-namespace recursionthm
+notation n` ↦ `l := option.get (lambda_defined n l)
 
-def d [pca α] : α := option.get (lambda_defined 0 (Λ 1, (var 0 * var 0 * var 1)))
+namespace recursion
 
-lemma dtot [pca α] (f : α) : option.is_some (d ⬝ f) :=
+def d [pca α] : α := 0 ↦ Λ 1, (var 0 * var 0 * var 1)
+
+lemma dtot [pca α] (f : α) : defined (d ⬝ f) :=
 begin
-  have e : d ⬝ f = code (Λ 0, (com f * com f * var 0)),
-  { change (d ⬝ f) with (↓d * ↓f), unfold d, simp [lam, code], },
+  have e : d ⬝ f = expr (Λ 0, (com f * com f * var 0)),
+  { change (d ⬝ f) with (↓d * ↓f), unfold d, simp [lam, expr], },
   rw e,
   exact (lambda_defined 0 _),
 end
@@ -132,46 +118,73 @@ end
 lemma diagonal [pca α] (f x : α) : d ⬝ f * x = f ⬝ f * x :=
 begin
   calc
-    d ⬝ f * ↓x = ↓d * ↓f * ↓x                                      :rfl
-    ...       = code (Λ 0, (Λ 1, (var 0 * var 0 * var 1))) * ↓f * ↓x : by { unfold d, simp, }
-    ...       = f ⬝ f * ↓x                                            : by { simp [lam, code], refl, }
+    d ⬝ f * ↓x = ↓d * ↓f * ↓x                                        :rfl
+    ...         = expr (Λ 0, (Λ 1, (var 0 * var 0 * var 1))) * ↓f * ↓x : by { unfold d, simp, }
+    ...         = f ⬝ f * ↓x                                            : by { simp [lam, expr], refl, }
 end
 
-def v [pca α] : α := option.get (lambda_defined 0 (Λ 1, (var 0 * (com d * var 1))))
-def n [pca α] : α := option.get (lambda_defined 0 (com d * (com v * var 0)))
+def v [pca α] : α := 0 ↦ Λ 1, (var 0 * (com d * var 1))
+def n [pca α] : α := 0 ↦ com d * (com v * var 0)
 
 theorem recursion [pca α] (f : α) : n ⬝ f ≃ f * (n ⬝ f) :=
 begin
   intros x,
-  let vf := option.get (lambda_defined 0 (com f * (com d * var 0))),  
-  have hv : ↓v * ↓f ↓= vf, { unfold v, simp [lam, code], },
+  let vf := (0 ↦ com f * (com d * var 0)),  
+  have hv : ↓v * ↓f ↓= vf, { unfold v, simp [lam, expr], },
   have nf_dvf : ↓n * ↓f = ↓d * ↓vf,
   { calc
-      ↓n * ↓f = code (Λ 0, (com d * (com v * var 0))) * ↓f : by { unfold n, simp, }
-      ...       = ↓d * ↓vf                                  : by { rw ← hv, simp [lam, code], } },
+      ↓n * ↓f = expr (Λ 0, (com d * (com v * var 0))) * ↓f : by { unfold n, simp, }
+      ...       = ↓d * ↓vf                                  : by { rw ← hv, simp [lam, expr], } },
   calc
     n ⬝ f * x = ↓n * ↓f * x          : rfl
     ...       = ↓d * ↓vf * x         : by { rw nf_dvf, }
     ...       = ↓vf * ↓vf * x        : diagonal vf x
-    ...       = ↓f * (↓d * ↓vf) * x : by { simp [lam, code], }
+    ...       = ↓f * (↓d * ↓vf) * x : by { simp [lam, expr], }
     ...       = ↓f * (↓n * ↓f) * x  : by { rw nf_dvf, }
 end
 
-theorem fixpoint_def [pca α] (f : α) : option.is_some (n ⬝ f) :=
+theorem ntot [pca α] (f : α) : defined (n ⬝ f) :=
 begin
-  let vf := option.get (lambda_defined 0 (com f * (com d * var 0))),  
-  have hv : ↓v * ↓f = ↓vf, { unfold v, simp [lam, code], },
+  let vf := (0 ↦ com f * (com d * var 0)),  
+  have hv : ↓v * ↓f = ↓vf, { unfold v, simp [lam, expr], },
   have nf_dvf : n ⬝ f = ↓d * ↓vf,
   { calc
-      ↓n * ↓f = code (Λ 0, (com d * (com v * var 0))) * ↓f : by { unfold n, simp, }
-      ...       = ↓d * ↓vf                                  : by { rw ← hv, simp [lam, code], } },
+      ↓n * ↓f = expr (Λ 0, (com d * (com v * var 0))) * ↓f : by { unfold n, simp, }
+      ...       = ↓d * ↓vf                                  : by { rw ← hv, simp [lam, expr], } },
   rw nf_dvf,
   exact (dtot _)
 end
 
-end recursionthm
+end recursion
 
-def fixpoint [pca α] : α := recursionthm.n
-def recursion  [pca α] (f : α) : fixpoint ⬝ f ≃ f * (fixpoint ⬝ f) := recursionthm.recursion f
+def fixpoint [pca α] : α := recursion.n
+def recursion  [pca α] (f x : α) : ↓fixpoint * ↓f * ↓x = f * (↓fixpoint * ↓f) * ↓x := recursion.recursion f x
+def fixpoint_of [pca α] (f : α) : α := option.get (recursion.ntot f)
 
+namespace calculation
+
+def pair [pca α] : α := 0 ↦ Λ 1, (Λ 2, (var 2 * var 0 * var 1))
+notation `⟪`a`, `b`⟫` := 0 ↦ var 0 * com a * com b
+def π₀ [pca α] : α := 0 ↦ var 0 * com k
+def π₁ [pca α] : α := 0 ↦ var 0 * (com k * com i)
+
+lemma pair_h [pca α] (a b : α) : ↓pair * ↓a * ↓b = ↓⟪a, b⟫ :=
+begin
+  calc
+    ↓pair * ↓a * ↓b = expr (Λ 0, (Λ 1, (Λ 2, (var 2 * var 0 * var 1)))) * ↓a * ↓b
+      : by { unfold pair, simp, }
+    ...                = expr (Λ 0, (var 0 * com a * com b))
+      : by {simp [lam, expr, if_neg (show 2 ≠ 0, from dec_trivial), if_neg (show 2 ≠ 1, from dec_trivial)], }
+    ...                = ↓⟪a, b⟫
+      : by { simp, },
+end
+
+lemma pair_pi0 [pca α] (a b : α) : ↓π₀ * ↓⟪a, b⟫ = ↓a := by { unfold π₀, simp [lam, expr], }
+lemma pair_pi1 [pca α] (a b : α) : ↓π₁ * ↓⟪a, b⟫ = ↓b := by { unfold π₁, simp [lam, expr], }
+
+end calculation
+
+
+def K [pca α] : set α := {x | defined (x ⬝ x)}
+def re_set [pca α] (A : set α) : Prop := ∃ e : α, A = {x | defined (e ⬝ x)}
 end pca
